comment out #eval, golf proofs in order.partitions

order/partitions.lean
@@ -26,13 +26,13 @@ lemma sub_of_gen_sub (x : α → α → Prop) (s : setoid α) (H : ∀ a b : α,
 
 def top : setoid α :=
 { r := λ s₁ s₂, true,
-  iseqv := by { unfold equivalence reflexive symmetric transitive,
-    exact ⟨by { intro, trivial }, by { intros, trivial }, by { intros, trivial }⟩ }}
+  iseqv := by unfold equivalence reflexive symmetric transitive;
+    exact ⟨λ _, trivial, λ _ _ _, trivial, λ _ _ _ _ _, trivial⟩ }
 
 def bot : setoid α :=
 { r := (=),
-  iseqv := by { unfold equivalence reflexive symmetric transitive,
-    exact ⟨by { intro, refl }, by { intros, exact a.symm }, by { intros, exact eq.trans a a_1 }⟩ }}
+  iseqv := by unfold equivalence reflexive symmetric transitive;
+    exact ⟨λ _, rfl, λ _ _ h, h.symm, λ _ _ _ h₁ h₂, eq.trans h₁ h₂⟩ }
 
 theorem eq_iff_r_eq : ∀ {r₁ r₂ : setoid α}, r₁ = r₂ ↔ r₁.r = r₂.r
 | ⟨r1, e1⟩ ⟨r2, e2⟩ :=
@@ -41,7 +41,7 @@ iff.intro (λ h, by injection h) (λ h, by dsimp at h; subst h)
 theorem eq_iff_eqv_class_eq {r₁ r₂ : setoid α} :
   r₁ = r₂ ↔ (∀ a, let r1 := r₁.r in let r2 := r₂.r in {b | r1 a b} = {b | r2 a b}) :=
 by rw eq_iff_r_eq; exact iff.intro (by { intros h a r1 r2, have : r1 = r2 := h, rw this })
-  ( λ h, by apply funext; exact h )
+  (λ h, by apply funext; exact h)
 
 instance : has_subset (setoid α) :=
 ⟨λ r₁ r₂, ∀ (a : α), let r1 := r₁.r in let r2 := r₂.r in {b | r1 a b} ⊆ {b | r2 a b}⟩
@@ -51,13 +51,12 @@ theorem subset_def (r₁ r₂ : setoid α) : r₁ ⊆ r₂ ↔ ∀ (a : α), let
 iff.rfl
 
 @[simp] theorem subset.refl (r : setoid α) : r ⊆ r :=
-by rw [subset_def]; exact assume _, set.subset.refl _
+by rw [subset_def]; exact λ _, set.subset.refl _
 
 theorem subset.trans {r₁ r₂ r₃ : setoid α} : r₁ ⊆ r₂ → r₂ ⊆ r₃ → r₁ ⊆ r₃ :=
-by iterate { rw [subset_def] }; exact assume h₁ h₂ a, set.subset.trans (h₁ a) (h₂ a)
+by iterate { rw [subset_def] }; exact λ h₁ h₂ a, set.subset.trans (h₁ a) (h₂ a)
 
-theorem subset.antisymm {r₁ r₂ : setoid α} (H₁ : r₁ ⊆ r₂) (H₂ : r₂ ⊆ r₁) :
-r₁ = r₂ :=
+theorem subset.antisymm {r₁ r₂ : setoid α} (H₁ : r₁ ⊆ r₂) (H₂ : r₂ ⊆ r₁) : r₁ = r₂ :=
 begin
   rw subset_def at H₁ H₂,
   rw eq_iff_eqv_class_eq,
@@ -65,7 +64,8 @@ begin
   exact set.subset.antisymm (H₁ a) (H₂ a)
 end
 
-instance : has_ssubset (setoid α) := ⟨λa b, a ⊆ b ∧ ¬ b ⊆ a⟩
+instance : has_ssubset (setoid α) :=
+⟨λa b, a ⊆ b ∧ ¬ b ⊆ a⟩
 
 def rel_union (r₁ r₂ : setoid α) : α → α → Prop :=
 λ s₁ s₂, let r1 := r₁.r in let r2 := r₂.r in r1 s₁ s₂ ∨ r2 s₁ s₂
@@ -76,8 +76,7 @@ eqv_gen.setoid $ rel_union r₁ r₂
 instance : has_union (setoid α) :=
 ⟨setoid.union⟩
 
-theorem union_def {r₁ r₂ : setoid α} : r₁ ∪ r₂ =
-eqv_gen.setoid (rel_union r₁ r₂) :=
+theorem union_def {r₁ r₂ : setoid α} : r₁ ∪ r₂ = eqv_gen.setoid (rel_union r₁ r₂) :=
 rfl
 
 @[simp] theorem subset_union_left (s t : setoid α) : s ⊆ s ∪ t :=
@@ -100,9 +99,10 @@ instance : has_inter (setoid α) :=
 ⟨setoid.inter⟩
 
 theorem inter_def {r₁ r₂ : setoid α} : r₁ ∩ r₂ =
-{ r := λ s₁ s₂, let r1 := r₁.r in let r2 := r₂.r in r1 s₁ s₂ ∧ r2 s₁ s₂,
-  iseqv := ⟨λ x, ⟨r₁.2.1 x, r₂.2.1 x⟩, (λ x y h, ⟨r₁.2.2.1 h.1, r₂.2.2.1 h.2⟩),
-      λ x y z h₁ h₂, ⟨r₁.2.2.2 h₁.1 h₂.1, r₂.2.2.2 h₁.2 h₂.2⟩⟩ } := rfl
+  { r := λ s₁ s₂, let r1 := r₁.r in let r2 := r₂.r in r1 s₁ s₂ ∧ r2 s₁ s₂,
+    iseqv := ⟨λ x, ⟨r₁.2.1 x, r₂.2.1 x⟩, (λ x y h, ⟨r₁.2.2.1 h.1, r₂.2.2.1 h.2⟩),
+      λ x y z h₁ h₂, ⟨r₁.2.2.2 h₁.1 h₂.1, r₂.2.2.2 h₁.2 h₂.2⟩⟩ } :=
+rfl
 
 @[simp] theorem inter_subset_left (r₁ r₂ : setoid α) : r₁ ∩ r₂ ⊆ r₁ :=
 by simp only [subset_def, set.subset_def]; exact λ a x h, and.left h
@@ -118,7 +118,8 @@ by simp only [subset_def, set.subset_def];
 exact λ a x h, trivial
 
 theorem bot_le (r : setoid α) : bot ⊆ r :=
-by simp only [subset_def, bot, set.subset_def, set.mem_set_of_eq]; exact λ a x h, h.symm ▸ (r.2.1 x)
+by simp only [subset_def, bot, set.subset_def, set.mem_set_of_eq];
+exact λ a x h, h.symm ▸ (r.2.1 x)
 
 def Sup (s : set (setoid α)) : setoid α :=
 eqv_gen.setoid $ λ (x y : α), ∃ r' : setoid α, r' ∈ s ∧ @r α r' x y
@@ -148,8 +149,8 @@ instance lattice_setoid : lattice.complete_lattice (setoid α) :=
 { lattice.complete_lattice .
   le           := (⊆),
   le_refl      := subset.refl,
-  le_trans     := assume a b c, subset.trans,
-  le_antisymm  := assume a b, subset.antisymm,
+  le_trans     := λ a b c, subset.trans,
+  le_antisymm  := λ a b, subset.antisymm,
 
   lt           := (⊂),
   lt_iff_le_not_le := λ x y, iff.refl _,
@@ -157,12 +158,12 @@ instance lattice_setoid : lattice.complete_lattice (setoid α) :=
   sup          := (∪),
   le_sup_left  := subset_union_left,
   le_sup_right := subset_union_right,
-  sup_le       := assume a b c, union_subset,
+  sup_le       := λ a b c, union_subset,
 
   inf          := (∩),
   inf_le_left  := inter_subset_left,
   inf_le_right := inter_subset_right,
-  le_inf       := assume a b c, subset_inter,
+  le_inf       := λ a b c, subset_inter,
 
   top          := top,
   le_top       := le_top,
@@ -181,7 +182,7 @@ instance lattice_setoid : lattice.complete_lattice (setoid α) :=
 variables (α) (𝔯 : setoid α)
 
 /- We define a partition as a family of nonempty sets such that any element of α is contained in
-exactly one set -/
+a unique set. -/
 
 /- Is there a way to set this up so that we talk about the equivalence classes via quot? -/
 structure partition :=
@@ -192,45 +193,30 @@ structure partition :=
 variable {α}
 
 theorem disjoint_union_of_partition (P : partition α) :
-set.sUnion P.1 = @set.univ α ∧
-∀ (b₁ b₂), b₁ ∈ P.1 → b₂ ∈ P.1 → b₁ ≠ b₂ → disjoint b₁ b₂ :=
-begin
-  simp [set.ext_iff],
-  split,
-  { intro a,
-      have hP := P.blocks_partition a,
-      exact exists.elim hP (by { intros b hb,
-        exact exists.intro b ⟨hb.1, hb.2.1⟩ }) },
-  { intros b₁ b₂ hb₁ hb₂ h,
+  set.sUnion P.1 = @set.univ α ∧ ∀ b₁ b₂, b₁ ∈ P.1 → b₂ ∈ P.1 → b₁ ≠ b₂ → disjoint b₁ b₂ :=
+by simp [set.ext_iff];
+  exact ⟨λ a, exists.elim (P.blocks_partition a) $ λ b hb, exists.intro b ⟨hb.1, hb.2.1⟩,
+  by { intros b₁ b₂ hb₁ hb₂ h,
     rw ←set.ext_iff at h,
     have HP : ∅ ∉ P.blocks := P.empty_not_mem_blocks,
-    have hP' := P.blocks_partition,
-    have Hb₁ : b₁ ≠ ∅ := by { intro h', exact (h'.symm ▸ HP) hb₁ },
+    have Hb₁ : b₁ ≠ ∅ := λ h', (h'.symm ▸ HP) hb₁,
     refine set.disjoint_left.mpr _,
     intros a ha,
-    replace hP' := hP' a,
-    exact exists.elim hP' (by { intros b' hb',
-      have Hb' : b' = b₁ := by { have := (hb'.2.2 b₁ hb₁), exact this ha }, intro h',
-      exact h (eq.trans Hb'.symm $ hb'.2.2 b₂ hb₂ $ Hb'.symm ▸ h') }) }
-end
+    exact exists.elim (P.blocks_partition a) (λ b' hb' h',
+      have Hb' : b₁ = b' := ((hb'.2.2 b₁ hb₁) ha).symm,
+      h (eq.trans Hb' $ hb'.2.2 b₂ hb₂ $ Hb' ▸ h')) }⟩
 
-def partition_of_disjoint_union {P : set (set α)} (h₁ : ∅ ∉ P)
-(h₂ : set.sUnion P = @set.univ α)
-(h₃ : ∀ (b₁ b₂), b₁ ∈ P → b₂ ∈ P → b₁ ≠ b₂ → disjoint b₁ b₂) : partition α :=
+def partition_of_disjoint_union {P : set (set α)} (h₁ : ∅ ∉ P) (h₂ : set.sUnion P = @set.univ α)
+  (h₃ : ∀ (b₁ b₂), b₁ ∈ P → b₂ ∈ P → b₁ ≠ b₂ → disjoint b₁ b₂) : partition α :=
 by simp [set.ext_iff] at h₂;
 exact { blocks := P,
   empty_not_mem_blocks := h₁,
-  blocks_partition := assume (a : α),
-    by replace h₂ : ∃ b, b ∈ P ∧ a ∈ b := h₂ a;
-    exact exists.elim h₂ (assume (b : set α)
-      (hb : b ∈ P ∧ a ∈ b),
-      and.elim hb $ assume (hb : b ∈ P) (hab : a ∈ b),
-        exists.intro b ⟨hb,hab,assume (b' : set α) (hb' : b' ∈ P) (hab' : a ∈ b'),
-          by { have := mt (h₃ b b' hb hb'), haveI := classical.prop_decidable,
-            simp at this, refine this (mt disjoint_iff.mp _),
-            change b ∩ b' ≠ ∅,
-            refine @set.ne_empty_of_mem _ (b ∩ b') a _,
-            exact set.mem_inter hab hab' }⟩) }
+  blocks_partition := λ a, by exact exists.elim (h₂ a) (λ b hb, and.elim hb $ λ hb hab,
+    exists.intro b ⟨hb, hab, λ b' hb' hab',
+      by { have : ¬disjoint b b' → ¬b ≠ b' := mt (h₃ b b' hb hb'),
+        haveI := classical.prop_decidable,
+        simp at this, refine this (mt disjoint_iff.mp _),
+        exact @set.ne_empty_of_mem _ (b ∩ b') a (set.mem_inter hab hab') }⟩) }
 
 namespace partition
 variables {α} (P : partition α)
@@ -248,153 +234,115 @@ ext.2
 
 theorem setoid_blocks_partition : ∀ a : α, ∃ b : set α, b ∈ {t | ∃ a : α, {b | a ≈ b} = t} ∧
   a ∈ b ∧ ∀ b' ∈ {t | ∃ a : α, {b | a ≈ b} = t}, a ∈ b' → b = b' :=
-let r' := 𝔯.r in
-  assume a, by { exact exists.intro {b | a ≈ b}
-    (by { split, { exact exists.intro a rfl },
-      { split, { simp },
-        { simp only [set.ext_iff, set.mem_set_of_eq],
-          intros x h₁ h₂ a',
-          exact exists.elim h₁ (by { intros y hy,
-            have ha : y ≈ a := (hy a).mpr h₂, have ha' : y ≈ a' ↔ a' ∈ x := hy a',
-            split, { intro H, exact ha'.mp (setoid.trans ha H) },
-            { intro H, exact setoid.trans (setoid.symm ha) (ha'.mpr H) } }) }}})}
+let r' := 𝔯.r in λ a, exists.intro {b | a ≈ b}
+  ⟨exists.intro a rfl, by simp,
+  by simp only [set.ext_iff, set.mem_set_of_eq];
+    exact λ x h₁ h₂ a', exists.elim h₁ $ λ y hy,
+      have ha : y ≈ a := (hy a).mpr h₂, have ha' : y ≈ a' ↔ a' ∈ x := hy a',
+      iff.intro (λ H, ha'.mp (setoid.trans ha H)) $
+        λ H, setoid.trans (setoid.symm ha) $ ha'.mpr H⟩
 
-/- There is a partition associated to an equivalence relation on a set -/
 def coe_of_setoid : partition α :=
 let r' := 𝔯.r in
 { blocks := {t | ∃ a, {b | a ≈ b} = t},
-  empty_not_mem_blocks := by { rw [set.nmem_set_of_eq], intro h,
-    exact exists.elim h (by { intros a ha, simp [set.eq_empty_iff_forall_not_mem] at ha,
-      exact ha a (setoid.refl a) }) },
+  empty_not_mem_blocks := by rw [set.nmem_set_of_eq]; exact λ h, exists.elim h
+    (λ a ha, by simp [set.eq_empty_iff_forall_not_mem] at ha; exact ha a (setoid.refl a)),
   blocks_partition := setoid_blocks_partition 𝔯 }
 
 def setoid_of_partition : setoid α :=
 { r := λ x y, ∃ b, b ∈ P.blocks ∧ x ∈ b ∧ y ∈ b,
   iseqv := ⟨λ x, exists.elim (P.blocks_partition x) (λ b h, exists.intro b ⟨h.1, h.2.1, h.2.1⟩),
-    λ x y H, exists.elim H (λ b hb, exists.intro b ⟨hb.1, hb.2.2, hb.2.1⟩),
+    λ x y H, exists.elim H $ λ b hb, exists.intro b ⟨hb.1, hb.2.2, hb.2.1⟩,
     λ x y z hxy hyz, exists.elim hxy $ λ b hb, exists.elim hyz $
       λ b' hb', exists.elim (P.blocks_partition y) $
-        λ b'' hb'', by { have Hb : b'' = b := hb''.2.2 b hb.1 hb.2.2,
+        λ b'' hb'', have Hb : b'' = b := hb''.2.2 b hb.1 hb.2.2,
           have Hb' : b'' = b' := hb''.2.2 b' hb'.1 hb'.2.1,
-          exact exists.intro b'' ⟨hb''.1, Hb.symm ▸ hb.2.1, Hb'.symm ▸ hb'.2.2⟩ }⟩ }
+          exists.intro b'' ⟨hb''.1, Hb.symm ▸ hb.2.1, Hb'.symm ▸ hb'.2.2⟩⟩ }
 
 theorem setoid_partition_setoid : setoid_of_partition (coe_of_setoid 𝔯) = 𝔯 :=
-begin
-  unfold setoid_of_partition coe_of_setoid,
-  simp [setoid.eq_iff_r_eq],
-  ext x y, split,
-  { intro H, exact exists.elim H (λ b hb, exists.elim hb.1
-    (by { intros a ha,
-    have hax : x ≈ a := by { have := ha.substr hb.2.1, rw [set.mem_set_of_eq] at this,
-      exact setoid.symm this },
-    have hay : y ≈ a := by { have := ha.substr hb.2.2, rw [set.mem_set_of_eq] at this,
-      exact setoid.symm this },
-    exact setoid.trans hax (setoid.symm hay) })) },
-  { intro H, exact exists.elim (setoid_blocks_partition 𝔯 x)
-    (by { intros b h, exact exists.intro b (⟨exists.intro x $ exists.elim h.1 $
-      λ y' hy', by { simp only [set.ext_iff, set.mem_set_of_eq] at hy' ⊢,
-        have Hy'x : y' ≈ x := (hy' x).mpr h.2.1,
-        intro a, split, { intro ha, exact (hy' a).mp (setoid.trans Hy'x ha) },
-        { intro ha, exact setoid.trans (setoid.symm Hy'x) ((hy' a).mpr ha) } },
-      h.2.1, exists.elim h.1 $ λ y' hy', by simp [set.ext_iff] at hy';
-        exact (hy' y).mp (setoid.trans ((hy' x).mpr h.2.1) H : y' ≈ y)⟩) }) }
-end
+by unfold setoid_of_partition coe_of_setoid; simp only [eq_iff_r_eq];
+ext x y;
+exact iff.intro
+(λ H, exists.elim H $ λ b hb, exists.elim hb.1 $ λ a ha,
+  have hax : x ≈ a := by { have := ha.substr hb.2.1, rw [set.mem_set_of_eq] at this,
+    exact setoid.symm this },
+  have hay : a ≈ y := by { have := ha.substr hb.2.2, rwa [set.mem_set_of_eq] at this },
+  setoid.trans hax $ hay)
+(λ H, exists.elim (setoid_blocks_partition 𝔯 x) $ λ b h, exists.intro b
+  ⟨exists.intro x $ exists.elim h.1 $ λ y' hy',
+    by simp only [set.ext_iff, set.mem_set_of_eq] at hy' ⊢;
+    exact λ a, have Hy'x : y' ≈ x := (hy' x).mpr h.2.1,
+      iff.intro (λ ha, (hy' a).mp $ setoid.trans Hy'x ha) $
+        λ ha, setoid.trans (setoid.symm Hy'x) $ (hy' a).mpr ha,
+  h.2.1, exists.elim h.1 $ λ y' hy', by simp only [set.ext_iff] at hy';
+    exact (hy' y).mp (setoid.trans ((hy' x).mpr h.2.1) H : y' ≈ y)⟩)
 
 theorem partition_setoid_partition : coe_of_setoid (setoid_of_partition P) = P :=
-begin
-  unfold setoid_of_partition coe_of_setoid,
-  simp [eq_of_blocks_eq],
-  ext x, split,
-  { intro H, simp only [set.mem_set_of_eq] at H,
-    exact exists.elim H (by { intros a ha,
-      replace ha : {y : α | ∃ (b : set α), b ∈ @blocks α P ∧ a ∈ b ∧ y ∈ b} = x := ha,
-      exact exists.elim (P.blocks_partition a)
-        (by { intros x' hx',
-          have : x = x' := by { rw ←ha,
-            ext y, rw [set.mem_set_of_eq], split,
-            { intro hy, exact exists.elim hy
-              (λ b' hb', (hx'.2.2 b' hb'.1 hb'.2.1).substr hb'.2.2) },
-            { intro hy, exact exists.intro x' ⟨hx'.1, hx'.2.1, hy⟩} },
-        exact this.symm ▸ hx'.1 }) }) },
-  { intro H, simp only [set.mem_set_of_eq],
-    change ∃ a, {y | ∃ b, b ∈ P.blocks ∧ a ∈ b ∧ y ∈ b} = x,
-    have xne : x ≠ ∅ := λ h, (h.symm ▸ P.empty_not_mem_blocks) H,
-    exact exists.elim (set.exists_mem_of_ne_empty xne) (by {
-      intros a ha,
-      exact exists.intro a (by { ext y, simp only [set.mem_set_of_eq],
-        split,
-        { intro hy, exact exists.elim hy
-          (by { intros b hb,
-            have := P.blocks_partition a,
-            exact exists.elim this
-              (by { intros b' hb',
-              have hb'b : b' = b := hb'.2.2 b hb.1 hb.2.1,
+by unfold setoid_of_partition coe_of_setoid; simp only [eq_of_blocks_eq];
+ext x; simp only [set.mem_set_of_eq];
+exact iff.intro
+  (λ H, exists.elim H $ λ a ha, exists.elim (P.blocks_partition a) $
+    λ x' hx', have x = x' := by rw ←ha;
+      ext y; rw [set.mem_set_of_eq];
+        exact iff.intro
+          (λ hy, exists.elim hy $ λ b' hb', (hx'.2.2 b' hb'.1 hb'.2.1).substr hb'.2.2)
+          (λ hy, exists.intro x' ⟨hx'.1, hx'.2.1, hy⟩),
+      this.symm ▸ hx'.1)
+  (λ H, have xne : x ≠ ∅ := λ h, (h.symm ▸ P.empty_not_mem_blocks) H,
+    exists.elim (set.exists_mem_of_ne_empty xne) $ λ a ha, exists.intro a $
+      by ext y; simp only [set.mem_set_of_eq];
+        exact iff.intro
+          (λ hy, exists.elim hy $ λ b hb, exists.elim (P.blocks_partition a)
+            (λ b' hb', have hb'b : b' = b := hb'.2.2 b hb.1 hb.2.1,
               have hb'x : b' = x := hb'.2.2 x H ha,
-              exact (eq.trans hb'b.symm hb'x).subst hb.2.2, }) }) },
-        { intro hy, exact exists.intro x ⟨H, ha, hy⟩ } }) }) }
-end
+              (eq.trans hb'b.symm hb'x).subst hb.2.2))
+          (λ hy, exists.intro x ⟨H, ha, hy⟩))
 
 instance : has_subset (partition α) :=
 ⟨λ P₁ P₂, ∀ p ∈ P₁.1, ∃ q, q ∈ P₂.1 ∧ p ⊆ q⟩
 
-theorem subset_def (P₁ P₂ : partition α) : P₁ ⊆ P₂ ↔ ∀ p ∈ P₁.1,
-∃ q, q ∈ P₂.1 ∧ p ⊆ q :=
+theorem subset_def (P₁ P₂ : partition α) : P₁ ⊆ P₂ ↔ ∀ p ∈ P₁.1, ∃ q, q ∈ P₂.1 ∧ p ⊆ q :=
 iff.rfl
 
 @[simp] theorem subset.refl (P : partition α) : P ⊆ P :=
-by rw [subset_def]; exact assume p H, exists.intro p ⟨H, set.subset.refl p⟩
+by rw [subset_def]; exact λ p H, exists.intro p ⟨H, set.subset.refl p⟩
 
 theorem subset.trans {s₁ s₂ s₃ : partition α} : s₁ ⊆ s₂ → s₂ ⊆ s₃ → s₁ ⊆ s₃ :=
-by iterate { rw subset_def };
-exact assume (h₁ : ∀ p ∈ s₁.1, ∃ q, q ∈ s₂.1 ∧ p ⊆ q)
-  (h₂ : ∀ p ∈ s₂.1, ∃ q, q ∈ s₃.1 ∧ p ⊆ q) (p : set α) (hp : p ∈ s₁.1),
-  exists.elim (h₁ p hp : ∃ q, q ∈ s₂.1 ∧ p ⊆ q)
-    (assume (p' : set α) (hp' : p' ∈ s₂.blocks ∧ p ⊆ p'),
-    exists.elim (h₂ p' hp'.1 : ∃ q, q ∈ s₃.1 ∧ p' ⊆ q) $
-      assume (p'' : set α) (hp'' : p'' ∈ s₃.blocks ∧ p' ⊆ p''),
-      exists.intro p'' ⟨hp''.1, set.subset.trans hp'.2 hp''.2⟩)
+by iterate { rw subset_def }; exact λ h₁ h₂ p hp, exists.elim (h₁ p hp)
+  (λ p' hp', exists.elim (h₂ p' hp'.1) $
+    λ p'' hp'', exists.intro p'' ⟨hp''.1, set.subset.trans hp'.2 hp''.2⟩)
 
-theorem subset.antisymm {s₁ s₂ : partition α} (H₁ : s₁ ⊆ s₂) (H₂ : s₂ ⊆ s₁) :
-s₁ = s₂ :=
+theorem subset.antisymm {s₁ s₂ : partition α} (H₁ : s₁ ⊆ s₂) (H₂ : s₂ ⊆ s₁) : s₁ = s₂ :=
 begin
   haveI := classical.prop_decidable,
-  rw subset_def at H₁ H₂,
   have hs₁ := disjoint_union_of_partition s₁, have hs₂ := disjoint_union_of_partition s₂,
-  ext,
-  exact iff.intro (assume (h : b ∈ s₁.blocks),
-    exists.elim (H₁ b h) $
-      assume (b' : set α) (hb' : b' ∈ s₂.blocks ∧ b ⊆ b'),
-      have ∃ q, q ∈ s₁.blocks ∧ b' ⊆ q := H₂ b' hb'.1,
-      exists.elim this $ by { assume (b'' : set α) (hb'' : b'' ∈ s₁.blocks ∧ b' ⊆ b''),
-        replace hs₁ := mt (hs₁.2 b b'' h hb''.1), simp at hs₁,
+  ext, rw subset_def at H₁ H₂,
+  exact iff.intro
+    (λ h, exists.elim (H₁ b h) $ λ b' hb', exists.elim (H₂ b' hb'.1) $ λ b'' hb'',
+      by { replace hs₁ := mt (hs₁.2 b b'' h hb''.1), simp at hs₁,
         have : b = b'' := by { refine hs₁ _,
           have : b ⊆ b'' := set.subset.trans hb'.2 hb''.2,
           have hinter : b ∩ b'' = b := set.inter_of_subset this,
           have hbne : b ≠ ∅ := by { by_contra H, simp at H,
             exact s₁.empty_not_mem_blocks (H ▸ h) },
-          replace hinter := hinter.substr hbne,
-          simp [disjoint], exact hinter },
+          replace hinter := hinter.substr hbne, simpa [disjoint] },
         have b'b : b' = b := set.subset.antisymm (this.symm ▸ hb''.2) (hb'.2),
         exact b'b ▸ hb'.1 })
-    (assume (h : b ∈ s₂.blocks), exists.elim (H₂ b h) $
-      assume (b' : set α) (hb' : b' ∈ s₁.blocks ∧ b ⊆ b'),
-      have ∃ q, q ∈ s₂.blocks ∧ b' ⊆ q := H₁ b' hb'.1,
-      exists.elim this $ by { assume (b'' : set α) (hb'' : b'' ∈ s₂.blocks ∧ b' ⊆ b''),
-        replace hs₂ := mt (hs₂.2 b b'' h hb''.1), simp at hs₂,
+    (λ h, exists.elim (H₂ b h) $ λ b' hb', exists.elim (H₁ b' hb'.1) $ λ b'' hb'',
+      by { replace hs₂ := mt (hs₂.2 b b'' h hb''.1), simp at hs₂,
         have : b = b'' := by { refine hs₂ _,
           have : b ⊆ b'' := set.subset.trans hb'.2 hb''.2,
           have hinter : b ∩ b'' = b := set.inter_of_subset this,
           have hbne : b ≠ ∅ := by { by_contra H, simp at H,
             exact s₂.empty_not_mem_blocks (H ▸ h) },
-          replace hinter := hinter.substr hbne,
-          simp [disjoint], exact hinter },
+          replace hinter := hinter.substr hbne, simpa [disjoint] },
         have b'b : b' = b := set.subset.antisymm (this.symm ▸ hb''.2) (hb'.2),
         exact b'b ▸ hb'.1 })
 end
 
-instance : has_ssubset (partition α) := ⟨λa b, a ⊆ b ∧ ¬ b ⊆ a⟩
+instance : has_ssubset (partition α) :=
+⟨λa b, a ⊆ b ∧ ¬ b ⊆ a⟩
 
-/- This instance sets up the poset structure on `partitions α` -/
 instance partial_order_of_partitions : partial_order (partition α) :=
 { le := (⊆),
   lt := (⊂),
@@ -406,42 +354,25 @@ set_option pp.implicit true
 
 theorem setoid_of_partition_order_preserving (s₁ s₂ : setoid α) :
   s₁ ⊆ s₂ ↔ coe_of_setoid s₁ ⊆ coe_of_setoid s₂ :=
-by { simp [coe_of_setoid, subset_def, setoid.subset_def, set.ext_iff, set.subset_def],
-    split,
-    { intros H p x hx,
-      exact exists.intro {x' | @r α s₂ x x'}
-        ⟨exists.intro x (by { intro y, replace hx : ∀ x', @r α s₁ x x' ↔ x' ∈ p := hx,
-          change @r α s₂ x y ↔ @r α s₂ x y, trivial }),
-        by { intros y hy, change @r α s₂ x y, exact H x y ((hx y).mpr hy) }⟩ },
-    { intros H x y hxy,
-      have := H {x' | @r α s₁ x x'} x (by { intro x', trivial }),
-      exact exists.elim this (by {
-        intros q hq,
-        have Hx : x ∈ q := hq.2 x (s₁.2.1 x),
-        have Hy : y ∈ q := hq.2 y hxy,
-        exact exists.elim hq.1 (by { intros a ha,
-          have hax : @r α s₂ a x := (ha x).mpr Hx,
-          have hay : @r α s₂ a y := (ha y).mpr Hy,
-          exact s₂.2.2.2 (s₂.2.2.1 hax) hay }) }) } }
+by simp [coe_of_setoid, subset_def, setoid.subset_def, set.ext_iff, set.subset_def];
+exact iff.intro
+  (λ H p x hx, exists.intro {x' | @r α s₂ x x'}
+    ⟨exists.intro x $ λ y, by trivial, λ y hy, H x y $ (hx y).mpr hy⟩)
+  (λ H x y hxy, exists.elim (H {x' | @r α s₁ x x'} x (λ x', by trivial)) $
+    λ q hq, have Hx : x ∈ q := hq.2 x (s₁.2.1 x), have Hy : y ∈ q := hq.2 y hxy,
+      exists.elim hq.1 $ λ a ha, have hax : @r α s₂ a x := (ha x).mpr Hx,
+        have hay : @r α s₂ a y := (ha y).mpr Hy, s₂.2.2.2 (s₂.2.2.1 hax) hay)
 
-lemma order_iso_setoid_partition : @order_iso (setoid α) (partition α) (⊆)
-  (⊆) :=
+lemma order_iso_setoid_partition : @order_iso (setoid α) (partition α) (⊆) (⊆) :=
 { to_fun := coe_of_setoid,
   inv_fun := setoid_of_partition,
   left_inv := setoid_partition_setoid,
   right_inv := partition_setoid_partition,
-  ord := by { intros s₁ s₂,
-    change s₁ ⊆ s₂ ↔ coe_of_setoid s₁ ⊆ coe_of_setoid s₂,
-    exact setoid_of_partition_order_preserving s₁ s₂ } }
+  ord := setoid_of_partition_order_preserving }
 
 theorem gc : coe_of_setoid 𝔯 ≤ P ↔ 𝔯 ≤ setoid_of_partition P :=
-begin
-  change coe_of_setoid 𝔯 ⊆ P ↔ 𝔯 ⊆ setoid_of_partition P,
-  have : coe_of_setoid 𝔯 ⊆ P ↔ coe_of_setoid 𝔯 ⊆ coe_of_setoid (setoid_of_partition P) :=
-    by rw partition_setoid_partition,
-  rw [setoid_of_partition_order_preserving],
-  rw this
-end
+calc _ ↔ coe_of_setoid 𝔯 ⊆ coe_of_setoid (setoid_of_partition P) : by rw partition_setoid_partition
+... ↔ 𝔯 ⊆ _ : by rw setoid_of_partition_order_preserving
 
 protected def galois_insertion : @galois_insertion (setoid α) (partition α) _ _
   (λ S, coe_of_setoid S) (λ P, setoid_of_partition P) :=
